check EC less

AwsCryptographicMaterialProviders/dafny/AwsCryptographicMaterialProviders/test/Keyrings/TestMultiKeyring.dfy
@@ -350,46 +350,8 @@ module TestMultiKeyring {
       && History in Modifies
     }
 
-    predicate OnEncryptEnsuresPublicly (
-      input: Types.OnEncryptInput ,
-      output: Result<Types.OnEncryptOutput, Types.Error> )
-      : (outcome: bool)
-      ensures
-        outcome ==>
-          output.Success?
-          ==>
-            && Materials.EncryptionMaterialsHasPlaintextDataKey(output.value.materials)
-            && Materials.ValidEncryptionMaterialsTransition(
-                 input.materials,
-                 output.value.materials
-               )
-    {
-      output.Success?
-      ==>
-        && Materials.EncryptionMaterialsHasPlaintextDataKey(output.value.materials)
-        && Materials.ValidEncryptionMaterialsTransition(
-             input.materials,
-             output.value.materials
-           )
-    }
-    predicate OnDecryptEnsuresPublicly ( input: Types.OnDecryptInput , output: Result<Types.OnDecryptOutput, Types.Error> )
-      : (outcome: bool)
-      ensures
-        outcome ==>
-          output.Success?
-          ==>
-            && Materials.DecryptionMaterialsTransitionIsValid(
-              input.materials,
-              output.value.materials
-            )
-    {
-      output.Success?
-      ==>
-        && Materials.DecryptionMaterialsTransitionIsValid(
-          input.materials,
-          output.value.materials
-        )
-    }
+    predicate OnEncryptEnsuresPublicly(input: Types.OnEncryptInput, output: Result<Types.OnEncryptOutput, Types.Error>) {true}
+    predicate OnDecryptEnsuresPublicly(input: Types.OnDecryptInput, output: Result<Types.OnDecryptOutput, Types.Error>){true}
 
     constructor(
       encryptionMaterials: Option<Types.EncryptionMaterials>,
@@ -448,46 +410,8 @@ module TestMultiKeyring {
       && History in Modifies
     }
 
-    predicate OnEncryptEnsuresPublicly (
-      input: Types.OnEncryptInput ,
-      output: Result<Types.OnEncryptOutput, Types.Error> )
-      : (outcome: bool)
-      ensures
-        outcome ==>
-          output.Success?
-          ==>
-            && Materials.EncryptionMaterialsHasPlaintextDataKey(output.value.materials)
-            && Materials.ValidEncryptionMaterialsTransition(
-                 input.materials,
-                 output.value.materials
-               )
-    {
-      output.Success?
-      ==>
-        && Materials.EncryptionMaterialsHasPlaintextDataKey(output.value.materials)
-        && Materials.ValidEncryptionMaterialsTransition(
-             input.materials,
-             output.value.materials
-           )
-    }
-    predicate OnDecryptEnsuresPublicly ( input: Types.OnDecryptInput , output: Result<Types.OnDecryptOutput, Types.Error> )
-      : (outcome: bool)
-      ensures
-        outcome ==>
-          output.Success?
-          ==>
-            && Materials.DecryptionMaterialsTransitionIsValid(
-              input.materials,
-              output.value.materials
-            )
-    {
-      output.Success?
-      ==>
-        && Materials.DecryptionMaterialsTransitionIsValid(
-          input.materials,
-          output.value.materials
-        )
-    }
+    predicate OnEncryptEnsuresPublicly(input: Types.OnEncryptInput, output: Result<Types.OnEncryptOutput, Types.Error>) {true}
+    predicate OnDecryptEnsuresPublicly(input: Types.OnDecryptInput, output: Result<Types.OnDecryptOutput, Types.Error>){true}
 
     constructor()
       ensures ValidState() && fresh(History) && fresh(Modifies)
